theories/iris/logrel/logrel_properties.v
@@ -11,6 +11,7 @@ From RichWasm Require Export layout syntax typing util.
 Require Export RichWasm.wasm.operations.
 From RichWasm.compiler Require Export prelude codegen instruction module.
 From RichWasm.iris Require Export autowp memory logrel util wp_codegen.
+From RichWasm.iris.logrel Require Export util.
 From RichWasm.iris.language Require Export cwp logpred.
 Require Export RichWasm.iris.logrel.instr.kinding.
 
@@ -341,6 +342,24 @@ Section properties.
     done.
   Qed.
 
+  Lemma atoms_interp_length os vs :
+    ⊢ atoms_interp os vs -∗ ⌜length os = length vs⌝.
+  Proof.
+    iApply big_sepL2_length.
+  Qed.
+
+  Lemma atoms_interp_one_inv o vs :
+    atoms_interp [o] vs ⊣⊢ ∃ v, ⌜vs = [v]⌝ ∗ atom_interp o v.
+  Proof.
+    iSplit.
+    - iIntros "Hvs".
+      iPoseProof (atoms_interp_cons_l with "Hvs") as (v vs' Heq) "[Hv Hnil]".
+      iPoseProof (atoms_interp_nil_l with "Hnil") as "->".
+      iExists v; auto.
+    - iIntros "(%v & -> & Hv)".
+      cbn; auto.
+  Qed.
+
   Lemma atom_interp_of_default ty :
     ⊢ ∃ o, atom_interp o (default_of_value_type ty).
   Proof.
@@ -429,6 +448,172 @@ Section properties.
       unfold ref_flag_atoms_interp, forall_satoms in Href_flag.
       by rewrite Forall_singleton in Href_flag.
   Qed.
+
+    Lemma atoms_interp_take os vs count :
+    atoms_interp os vs -∗
+    atoms_interp (take count os) (take count vs) ∗
+    atoms_interp (drop count os) (drop count vs).
+  Proof.
+    iIntros "Hatoms".
+    iDestruct (big_sepL2_length with "Hatoms") as %Hlen.
+    rewrite -{1}(take_drop count os) -{1}(take_drop count vs).
+    iDestruct (big_sepL2_app_inv with "Hatoms") as "[Htake Hdrop]".
+    { rewrite !length_take. lia. }
+    iFrame.
+  Qed.
+
+  Lemma atoms_interp_take_drop os vs off count :
+    atoms_interp os vs -∗
+    atoms_interp (take count (drop off os)) (take count (drop off vs)).
+  Proof.
+    iIntros "Hatoms".
+    iDestruct (atoms_interp_take with "Hatoms") as "[_ Hdrop]".
+    by iDestruct (atoms_interp_take with "Hdrop") as "[Htake_drop _]".
+  Qed.
+
+  Lemma atoms_interp_app_split_l os1 os2 vs1 vs2 :
+    length os1 = length vs1 ->
+    atoms_interp (os1 ++ os2) (vs1 ++ vs2) -∗
+    atoms_interp os1 vs1 ∗
+    atoms_interp os2 vs2.
+  Proof.
+    iIntros (Hlen) "Hatoms".
+    iDestruct (atoms_interp_take _ _ (length os1) with "Hatoms") as "[H1 H2]".
+    rewrite !take_app_length !drop_app_length Hlen !take_app_length !drop_app_length.
+    iFrame.
+  Qed.
+
+  Lemma atoms_interp_app_split_r os1 os2 vs1 vs2 :
+    atoms_interp os1 vs1 -∗
+    atoms_interp os2 vs2 -∗
+    atoms_interp (os1 ++ os2) (vs1 ++ vs2).
+  Proof.
+    iIntros "H1 H2".
+    iApply (big_sepL2_app with "H1 H2").
+  Qed.
+
+  Lemma atoms_interp_app_l os1 os2 vs :
+    atoms_interp (os1 ++ os2) vs -∗
+    ∃ vs1 vs2, ⌜vs = vs1 ++ vs2⌝ ∗ atoms_interp os1 vs1 ∗ atoms_interp os2 vs2.
+  Proof.
+    iIntros "Hos".
+    iDestruct (atoms_interp_length with "Hos") as %Hlen.
+    iDestruct (atoms_interp_take _ _ (length os1) with "Hos") as "[Hos1 Hos2]".
+    iEval (rewrite take_app_length) in "Hos1".
+    iEval (rewrite drop_app_length) in "Hos2".
+    iExists (take (length os1) vs), (drop (length os1) vs).
+    iSplit.
+    - iPureIntro. rewrite take_drop. reflexivity.
+    - iFrame.
+  Qed.
+
+  Lemma atoms_interp_app_r (os : list atom) (vs1 vs2 : list value) :
+    atoms_interp os (vs1 ++ vs2) -∗
+    ∃ os1 os2 : list atom, ⌜os = os1 ++ os2⌝ ∗ atoms_interp os1 vs1 ∗ atoms_interp os2 vs2.
+  Proof.
+    iIntros "Hos".
+    iDestruct (atoms_interp_length with "Hos") as %Hlen.
+    iDestruct (atoms_interp_take _ _ (length vs1) with "Hos") as "[Hos1 Hos2]".
+    iEval (rewrite take_app_length) in "Hos1".
+    iEval (rewrite drop_app_length) in "Hos2".
+    iExists (take (length vs1) os), (drop (length vs1) os).
+    iSplit.
+    - iPureIntro. rewrite take_drop. reflexivity.
+    - iFrame.
+  Qed.
+
+  Definition value_to_atom (v : value) : atom :=
+    match v with
+    | VAL_int32 n32 => I32A n32
+    | VAL_int64 n64 => I64A n64
+    | VAL_float32 f32 => F32A f32
+    | VAL_float64 f64 => F64A f64
+    end.
+
+  Definition values_to_atoms (vs : list value) :=
+    map value_to_atom vs.
+
+  Lemma atom_interp_value_as_atom v :
+    ⊢ atom_interp (value_to_atom v) v.
+  Proof.
+    destruct v; simpl; by iIntros.
+  Qed.
+
+  Lemma atoms_interp_values_as_atoms vs :
+   ⊢ atoms_interp (values_to_atoms vs) vs.
+  Proof.
+    iInduction vs as [|v vs] "IH"; first by simpl.
+    rewrite /values_to_atoms map_cons.
+    rewrite atoms_interp_cons.
+    iFrame "#".
+    iApply atom_interp_value_as_atom.
+  Qed.
+
+  Definition expect_heap_ptr (o : atom) : option (base_memory * location) :=
+    match o with
+    | PtrA (PtrHeap μ ℓ) => Some (μ, ℓ)
+    | _ => None
+    end.
+
+  Lemma atom_interp_dup o v :
+    expect_heap_ptr o = None ->
+    Persistent (atom_interp o v).
+  Proof.
+    destruct o; cbn; intros Heq; try apply bi.pure_persistent.
+    repeat (apply bi.pure_persistent
+    || (apply bi.exist_persistent; intros ?x)
+    || apply bi.sep_persistent).
+    destruct p; try congruence.
+    destruct x1; cbn;
+    repeat (apply bi.pure_persistent
+    || (apply bi.exist_persistent; intros ?x)
+    || apply bi.sep_persistent).
+  Qed.
+
+  Lemma atoms_interp_dup os vs :
+    Forall (λ o, expect_heap_ptr o = None) os ->
+    Persistent (atoms_interp os vs).
+  Proof.
+    intros Hall.
+    unfold atoms_interp.
+    apply big_sepL2_persistent.
+    intros k o v Hok Hvk.
+    apply atom_interp_dup.
+    rewrite Forall_lookup in Hall.
+    exact (Hall k o Hok).
+  Qed.
+
+  Global Instance atom_interp_value_to_atom_persistent v :
+    Persistent (atom_interp (value_to_atom v) v).
+  Proof.
+    unfold Persistent.
+    iIntros "H !>".
+    iApply atom_interp_value_as_atom.
+  Qed.
+
+  Global Instance atoms_interp_values_to_atoms_persistent vs :
+    Persistent (atoms_interp (values_to_atoms vs) vs).
+  Proof.
+    unfold Persistent.
+    iIntros "H !>".
+    iApply atoms_interp_values_as_atoms.
+  Qed.
+
+  Lemma atoms_interp_norefs_persistent (se: semantic_env (Σ:=Σ)) os vs :
+    ref_flag_atoms_interp NoRefs (SAtoms os) ->
+    Persistent (atoms_interp os vs).
+  Proof.
+    intros Href.
+    unfold ref_flag_atoms_interp, forall_satoms in Href.
+    apply atoms_interp_dup.
+    rewrite Forall_lookup. intros k o Hok.
+    rewrite Forall_lookup in Href.
+    specialize (Href k o Hok).
+    destruct o; simpl in *; try done.
+    destruct p; simpl in *; done.
+  Qed.
+
+
 
   Lemma frame_interp_wl_interp se F L WL ηss fr :
     frame_interp rti sr se ηss L WL fr -∗
@@ -728,24 +913,6 @@ Section properties.
     eapply frame_rel_Forall2_update; try done.
   Qed.
 
-  Lemma atoms_interp_length os vs :
-    ⊢ atoms_interp os vs -∗ ⌜length os = length vs⌝.
-  Proof.
-    iApply big_sepL2_length.
-  Qed.
-
-  Lemma atoms_interp_one_inv o vs :
-    atoms_interp [o] vs ⊣⊢ ∃ v, ⌜vs = [v]⌝ ∗ atom_interp o v.
-  Proof.
-    iSplit.
-    - iIntros "Hvs".
-      iPoseProof (atoms_interp_cons_l with "Hvs") as (v vs' Heq) "[Hv Hnil]".
-      iPoseProof (atoms_interp_nil_l with "Hnil") as "->".
-      iExists v; auto.
-    - iIntros "(%v & -> & Hv)".
-      cbn; auto.
-  Qed.
-
   Lemma value_interp_ref_sz se κ μ τ os :
     value_interp rti sr se (RefT κ μ τ) (SAtoms os) -∗ ⌜length os = 1⌝.
   Proof.
@@ -808,5 +975,450 @@ Section properties.
   Qed.
 
 
+  Lemma has_prim_has_arep η v :
+    has_prim η v ->
+    has_arep (prim_to_arep η) (value_to_atom v).
+  Proof.
+    intros Hprim.
+    destruct v, η; simpl; done.
+  Qed.
+
+  Lemma has_prims_has_areps ηs vs :
+    has_prims ηs vs ->
+    has_areps (map prim_to_arep ηs) (SAtoms (values_to_atoms vs)).
+  Proof.
+    revert ηs.
+    induction vs; intros ηs Hprims.
+    - inversion Hprims; subst.
+      simpl.
+      eexists.
+      by split.
+    - destruct ηs as [| η ηs]; first inversion Hprims.
+      simpl.
+      apply has_areps_cons.
+      apply Forall2_cons in Hprims as [Hprim Hprims].
+      split; first by apply IHvs.
+      by apply has_prim_has_arep.
+  Qed.
+
+  Lemma values_to_atoms_norefs vs :
+    Forall (forall_ptr_atom norefs_ptr_interp) (values_to_atoms vs).
+  Proof.
+    induction vs as [|v vs]; simpl; first done.
+    apply Forall_cons.
+    split.
+    - by destruct v.
+    - apply IHvs.
+  Qed.
+
+  Lemma locals_interp_lookup se L oss i τ_old :
+    L !! i = Some τ_old →
+    locals_interp rti sr se L oss -∗
+    ∃ oss_pre os_mid oss_post,
+    ⌜oss = oss_pre ++ [os_mid] ++ oss_post⌝ ∗
+    locals_interp rti sr se (take i L) oss_pre ∗
+    value_interp rti sr se τ_old (SAtoms os_mid) ∗
+    locals_interp rti sr se (drop (S i) L) oss_post.
+  Proof.
+    iIntros (Hlookup_L) "Hval".
+    iDestruct (big_sepL2_length with "Hval") as %Hoss_len.
+    have Hlookup_oss_i : ∃ os_mid, oss !! i = Some os_mid.
+    {
+      apply lookup_lt_is_Some_2.
+      rewrite -Hoss_len.
+      by eapply lookup_lt_Some.
+    }
+    destruct Hlookup_oss_i as [os_mid Hlookup_oss_i].
+    iExists (take i oss), os_mid, (drop (S i) oss).
+    iSplit.
+    { iPureIntro. symmetry. apply take_drop_middle. exact Hlookup_oss_i. }
+    (* unfold locals_interp. *)
+    have Hsplit_L := take_drop_middle L i τ_old Hlookup_L.
+    have Hsplit_oss := take_drop_middle oss i os_mid Hlookup_oss_i.
+    rewrite <- Hsplit_L, <- Hsplit_oss.
+    iDestruct (big_sepL2_app_inv with "Hval") as "[Hval_pre Hval_rest]".
+    { left. rewrite !length_take. lia. }
+    rewrite Hsplit_L Hsplit_oss.
+    iDestruct "Hval_rest" as "[Hval_mid Hval_post]".
+    unfold locals_interp.
+    iFrame.
+  Qed.
+
+  Lemma locals_interp_length se L oss :
+    locals_interp rti sr se L oss -∗ ⌜length L = length oss⌝.
+  Proof.
+    iIntros "Hval".
+    unfold locals_interp.
+    iDestruct (big_sepL2_length with "Hval") as %Hlen.
+    iPureIntro. exact Hlen.
+  Qed.
+
+  Lemma frame_interp_update_frame se ηss L wl1 wl2 wl vs_idxs vs_wl fr fr' :
+    vs_idxs = seq ((length $ concat ηss) + length wl1) (length wl) ->
+    Forall2 (λ i v, f_locs fr' !! i = Some v) vs_idxs vs_wl ->
+    result_type_interp wl vs_wl ->
+    frame_rel (λ i, i ∉ vs_idxs) fr fr' ->
+    frame_interp rti sr se ηss L (wl1 ++ wl ++ wl2) fr -∗
+    frame_interp rti sr se ηss L (wl1 ++ wl ++ wl2) fr'.
+  Proof.
+    intros Hvs_idxs_wl Hnew_vals Hres Hfrel.
+    iIntros "Hframe".
+    iDestruct "Hframe" as
+      "(%oss & %vss_L & %vs_WL_old & %Hfr & %Hprims & %Hresult & Hatom & Hval)".
+    apply result_type_interp_split in Hresult.
+    destruct Hresult as [vs_wl1 [vs_rest [-> [Hvs_wl1 Hresult]]]].
+    apply result_type_interp_split in Hresult.
+    destruct Hresult as [vs_wl' [vs_wl2 [-> [Hvs_wl' Hvs_wl2]]]].
+    iFrame.
+    iExists (vs_wl1 ++ vs_wl ++ vs_wl2).
+    iPureIntro; split; last split.
+    - rewrite app_assoc.
+      eapply (frame_f_locs_update); [ | done | done | by rewrite -app_assoc].
+      rewrite length_app.
+      apply Forall2_length in Hvs_wl' as <-.
+      apply Forall2_length in Hvs_wl1 as <-.
+      apply Forall2_concat in Hprims.
+      apply Forall2_length in Hprims as <-.
+      done.
+    - done.
+    - apply result_type_interp_combine; first done.
+      by apply result_type_interp_combine; last done.
+  Qed.
+
+  Lemma frame_interp_update_frame' se ηss L wl1 wl2 wl vs_localidxs vs_idxs vs_wl fr fr' :
+    vs_idxs = seq ((length $ concat ηss) + length wl1) (length wl) ->
+    vs_localidxs = map prelude.W.Mk_localidx vs_idxs ->
+    Forall2 (λ i v, f_locs fr' !! localimm i = Some v) vs_localidxs vs_wl ->
+    result_type_interp wl vs_wl ->
+    frame_rel (λ i, i ∉ vs_idxs) fr fr' ->
+    frame_interp rti sr se ηss L (wl1 ++ wl ++ wl2) fr -∗
+    frame_interp rti sr se ηss L (wl1 ++ wl ++ wl2) fr'.
+  Proof.
+    iIntros (Hvs_idxs Hvs_localidxs HF Hres Hframe_rel) "Hfr".
+    iApply frame_interp_update_frame; eauto.
+    subst vs_localidxs.
+    rewrite Forall2_fmap_l in HF.
+    eapply Forall2_impl; [exact HF|].
+    done.
+  Qed.
+
+  Lemma frame_interp_locals_ctx_length se ηss L WL fr :
+    frame_interp rti sr se ηss L WL fr -∗ ⌜length ηss = length L⌝.
+  Proof.
+    iIntros "Hframe".
+    iDestruct "Hframe" as (oss vss_L vs_WL Hf_locs Hhas_prims Hresult) "[Hatom Hval]".
+    iDestruct (locals_interp_length with "Hval") as "->".
+    iDestruct (big_sepL2_length with "Hatom") as "%Hoss_len".
+    iPureIntro.
+    apply Forall2_length in Hhas_prims as ->.
+    done.
+  Qed.
+
+  Lemma frame_interp_update_frame_label se τ_old ηs L wl vs_l vs_idxs os fe fr fr' i τ :
+    let L' := <[i:=τ]> L in
+    L !! i = Some τ_old ->
+    wl_interp (fe_wlocal_offset fe) wl fr ->
+    fe_locals fe !! i = Some ηs ->
+    vs_idxs = seq (sum_list_with length (take i (fe_locals fe))) (length ηs) ->
+    has_prims ηs vs_l ->
+    Forall2 (λ j v, f_locs fr' !! j = Some v) vs_idxs vs_l ->
+    frame_rel (λ j, j ∉ vs_idxs) fr fr' ->
+    atoms_interp os vs_l -∗
+    value_interp rti sr se τ (SAtoms os) -∗
+    frame_interp rti sr se (fe_locals fe) L wl fr -∗
+    frame_interp rti sr se (fe_locals fe) L' wl fr'.
+  Proof.
+    intros L' Hlookup_L Hwl_interp Hlookup Hvs_idxs Hhas_prims_new Hf2 Hfrel.
+    iIntros "Hatoms_new Hvalues Hframe".
+
+    iDestruct (frame_interp_locals_ctx_length with "Hframe") as "%HL_len".
+
+    iDestruct "Hframe" as
+      "(%oss & %vss_L & %vs_WL & %Hfr & %Hhas_prims & %Hresult & Hatoms & Hval)".
+    iFrame (Hresult).
+
+    have Hsplit := take_drop_middle (fe_locals fe) i ηs Hlookup.
+    rewrite <- Hsplit in Hhas_prims.
+    apply List.Forall2_app_inv_l in Hhas_prims as (vss_L_pre & vss_L_rest & Hpre & Hrest & ->).
+    destruct vss_L_rest as [| vs_mid vss_L_post]; [inversion Hrest |].
+    apply Forall2_cons_1 in Hrest as [Hmid Hpost].
+
+    iDestruct (locals_interp_lookup _ _ _ _ _ Hlookup_L with "Hval") as (oss_pre os_mid oss_post Hoss_eq) "[Hval_pre [_ Hval_post]]".
+
+    iEval (rewrite Hoss_eq) in "Hatoms".
+    iDestruct (locals_interp_length with "Hval_pre") as %Hlen_pre.
+    iDestruct (locals_interp_length with "Hval_post") as %Hlen_post.
+    apply Forall2_length in Hpre as Hvs_pre_len.
+    apply Forall2_length in Hmid as Hvs_mid_len.
+    apply Forall2_length in Hpost as Hvs_post_len.
+
+    have Hlen_oss_pre : length oss_pre = length vss_L_pre.
+    { rewrite <- Hlen_pre, length_take, <- Hvs_pre_len, length_take. lia. }
+    have Hlen_oss_post : length oss_post = length vss_L_post.
+    { rewrite <- Hlen_post, length_drop, <- Hvs_post_len, length_drop. lia. }
+
+    iDestruct (big_sepL2_app_inv _ _ _ _ _ with "Hatoms") as "[Hatoms_pre Hatoms_rest]"; first by left.
+    (* NOTE: the atoms_interp for the middle is being thrown away, since the values are being overwritten *)
+    iDestruct (big_sepL2_cons with "Hatoms_rest") as "[_ Hatoms_post]".
+
+    iExists (oss_pre ++ [os] ++ oss_post), (vss_L_pre ++ [vs_l] ++ vss_L_post).
+    iSplit.
+    {
+      iPureIntro.
+      rewrite !concat_app.
+      rewrite concat_app concat_cons in Hfr.
+      rewrite -!app_assoc.
+      rewrite -!app_assoc in Hfr.
+      clear_nils.
+      eapply frame_f_locs_update.
+      4: apply Hfr.
+      3: done.
+      2: done.
+      subst vs_idxs.
+      f_equal; last done.
+      rewrite -sum_list_with_length_concat.
+      eapply Forall2_sum_list_with_length.
+      eapply Forall2_impl; [exact Hpre |].
+      intros ηs' vs' Hprims'.
+      apply Forall2_length in Hprims'.
+      done.
+    }
+    iSplit.
+    {
+      iPureIntro.
+      rewrite <- (take_drop_middle (fe_locals fe) i ηs Hlookup).
+      apply Forall2_app; [exact Hpre |].
+      apply Forall2_cons; by split.
+    }
+    iSplitL "Hatoms_new Hatoms_pre Hatoms_post".
+    - by iFrame.
+    - unfold locals_interp, L'.
+      rewrite insert_take_drop.
+      2: { eapply lookup_lt_Some. exact Hlookup_L. }
+      iApply (big_sepL2_app with "Hval_pre").
+      iApply big_sepL2_cons.
+      iFrame.
+  Qed.
+
+  Lemma frame_interp_update_frame_label' se τ_old ηs L wl vs_l vs_idxs vs_localidxs os fe fr fr' i τ :
+    let L' := <[i:=τ]> L in
+    L !! i = Some τ_old ->
+    wl_interp (fe_wlocal_offset fe) wl fr ->
+    fe_locals fe !! i = Some ηs ->
+    vs_idxs = seq (sum_list_with length (take i (fe_locals fe))) (length ηs) ->
+    vs_localidxs = map prelude.W.Mk_localidx vs_idxs ->
+    has_prims ηs vs_l ->
+    Forall2 (λ j v, f_locs fr' !! localimm j = Some v) vs_localidxs vs_l ->
+    frame_rel (λ j, j ∉ vs_idxs) fr fr' ->
+    atoms_interp os vs_l -∗
+    value_interp rti sr se τ (SAtoms os) -∗
+    frame_interp rti sr se (fe_locals fe) L wl fr -∗
+    frame_interp rti sr se (fe_locals fe) L' wl fr'.
+  Proof.
+    intros L' HlookupL Hwl_interp Hlookup Hvs_idxs Hvs_localidxs Hhas_prims_new Hf2 Hfrel.
+    iIntros "Hatoms Hvalues Hframe".
+    iApply (frame_interp_update_frame_label with "[$] [$] [$]" ); eauto.
+    subst vs_localidxs.
+    rewrite Forall2_fmap_l in Hf2.
+    eapply Forall2_impl; [exact Hf2|].
+    done.
+  Qed.
+
+  Lemma atom_interp_value_type_interp (ι : atomic_rep) (o : atom) (v : value) :
+    has_arep ι o →
+    atom_interp o v -∗
+    ⌜value_type_interp (translate_arep ι) v⌝.
+  Proof.
+    intros Harep.
+    destruct ι, o; simpl in *; try done.
+    {
+      iIntros "(%n & %n32 & %Hrep & -> & _)".
+      iExists _; eauto.
+    }
+    all: iIntros "->"; iPureIntro; exists n; done.
+  Qed.
+
+  Lemma result_type_interp_of_atoms_interp ιs os vs :
+    has_areps ιs (SAtoms os) ->
+    atoms_interp os vs -∗
+    ⌜result_type_interp (map translate_arep ιs) vs⌝.
+  Proof.
+    revert os vs.
+    induction ιs as [| ι ιs' IH]; intros os vs Hιs'.
+    - (* ιs = [] *)
+      destruct Hιs' as (os' & Heq & Hfa).
+      inversion Heq; subst.
+      inversion Hfa; subst.
+      iIntros "Hinterp".
+      iDestruct (atoms_interp_nil_l with "Hinterp") as "->".
+      iPureIntro.
+      constructor.
+    - (* ιs = ι :: ιs' *)
+      destruct os as [| o os].
+      {
+        destruct Hιs' as (os' & Heq & Hfa).
+        inversion Heq; subst.
+        inversion Hfa.
+      }
+      apply has_areps_cons in Hιs' as [Hιs'_tl Hιs'_hd].
+      iIntros "Hinterp".
+      iDestruct (atoms_interp_cons_l with "Hinterp") as
+      "(%v & %vs' & -> & Hv & Hos)".
+      iDestruct (IH _ _ Hιs'_tl with "Hos") as "%Htl".
+      iDestruct (atom_interp_value_type_interp ι o v Hιs'_hd with "Hv") as "%Hhd".
+      iPureIntro.
+      simpl.
+      by constructor.
+  Qed.
+
+  Lemma value_type_interp_of_default ty :
+    value_type_interp ty (default_of_value_type ty).
+  Proof. destruct ty; by eexists. Qed.
+
+  Lemma result_type_interp_of_defaults tys :
+    result_type_interp tys (default_of_value_types tys).
+  Proof.
+    induction tys as [| ty tys IH].
+    - constructor.
+    - constructor; last done.
+      apply value_type_interp_of_default.
+  Qed.
+
+  Lemma empty_closure_interp se ϕ cl :
+    closure_interp rti sr ϕ senv_empty cl -∗
+    closure_interp rti sr ϕ se cl.
+  Proof.
+    (* This seems true? *)
+    iIntros "H".
+    cbn.
+  Admitted.
+
+
+  Lemma skind_rec_interp_unfold sκ T (se: semantic_env (Σ:=Σ)) sv :
+    skind_rec_interp sκ T se sv ≡ (▷ T (senv_insert_type sκ (skind_rec_interp sκ T se) se) sv)%I.
+  Proof.
+    simpl.
+    set f := (λ T0 : leibnizO semantic_value -n> iPropO Σ, λne sv0 : leibnizO semantic_value, (▷ T (se.1, (sκ, T0) :: se.2) sv0)%I).
+     etransitivity.
+     - exact (fixpoint_unfold f sv).
+     - simpl. reflexivity.
+  Qed.
+
+  Lemma rec_interp_unfold κ T (se: semantic_env (Σ:=Σ)) sv :
+    rec_interp κ T se sv ≡
+    match eval_kind_se se κ with
+    | Some sκ => ▷ T (senv_insert_type sκ (skind_rec_interp sκ T se) se) sv
+    | None => False
+    end%I.
+  Proof.
+    unfold rec_interp. simpl.
+    destruct (eval_kind se κ) as [sκ|]; simpl.
+    - set f := (λ T0 : leibnizO semantic_value -n> iPropO Σ,
+      λne sv0 : leibnizO semantic_value,
+      (▷ T (se.1, (sκ, T0) :: se.2) sv0)%I).
+      etransitivity.
+      + exact (fixpoint_unfold f sv).
+      + simpl. reflexivity.
+    - reflexivity.
+  Qed.
+
+  Lemma value_interp_type_plug se vs ηs :
+    ⌜has_prims ηs vs⌝ -∗
+    value_interp rti sr se (type_plug_prim ηs) (SAtoms (values_to_atoms vs)).
+  Proof.
+    iIntros "%Hprims".
+    rewrite value_interp_eq /add_skind_interp.
+    unfold type_plug_prim, type_plug. simpl.
+    set ρ := ProdR (map (AtomR ∘ prim_to_arep) ηs).
+    have Heval : eval_rep se ρ = Some (map prim_to_arep ηs).
+    { apply eval_rep_prod_atoms. }
+    iExists (SVALTYPE (map prim_to_arep ηs) NoRefs).
+    iSplit.
+    - iPureIntro. unfold type_skind. simpl.
+      have Heval_kind := eval_kind_of_eval_rep se ρ _ Heval NoRefs.
+      rewrite -Heval_kind.
+      done.
+    - apply has_prims_has_areps in Hprims as Hareps.
+      iSplit.
+      + iPureIntro. simpl.
+        split; first done.
+        apply values_to_atoms_norefs.
+      + iExists (map prim_to_arep ηs).
+        iSplit; [iPureIntro; exact Heval |].
+        done.
+  Qed.
+
+  Lemma type_interp_skind_svalue (τ : type) se sv :
+    type_interp rti sr τ se sv -∗ ∃ sκ, ⌜type_skind se τ = Some sκ⌝ ∗ ⌜skind_has_svalue sκ sv⌝.
+  Proof.
+    iIntros "H".
+    rewrite type_interp_eq.
+    iDestruct "H" as (sκ) "[%Hsk [%Hsv _]]".
+    iExists sκ. by iSplit; iPureIntro.
+  Qed.
+
+  (* TODO: might need to change. @Elan *)
+  Lemma fold_type_interp_subst (se : semantic_env (Σ:=Σ)) (τ : type) (κ : kind) sκ sv :
+    eval_kind se κ = Some sκ →
+    type_interp rti sr (subst_type VarM VarR VarS (unscoped.scons (RecT κ τ) VarT) τ) se sv ⊣⊢
+    type_interp rti sr τ (senv_insert_type sκ (skind_rec_interp sκ (type_interp rti sr τ) se) se) sv.
+  Proof. Admitted.
+
+  Lemma fold_type_interp (se : semantic_env (Σ:=Σ)) (τ : type) (κ : kind) sκ sv :
+    eval_kind se κ = Some sκ →
+    type_interp rti sr (RecT κ τ) se sv ⊣⊢
+    ⌜skind_has_svalue sκ sv⌝ ∗
+    ▷ type_interp rti sr (subst_type VarM VarR VarS (unscoped.scons (RecT κ τ) VarT) τ) se sv.
+  Proof.
+    intros Hκ.
+    iSplit.
+    - iIntros "H".
+      iEval (rewrite type_interp_eq) in "H".
+      iDestruct "H" as "(%sκ' & %Hκ' & %Hsv & Hrec)".
+      unfold type_skind in Hκ'. simpl in Hκ'.
+      rewrite Hκ in Hκ'. simplify_eq.
+      iSplit; first done.
+      iEval (cbn [pre_type_interp]) in "Hrec".
+      iEval (rewrite (rec_interp_unfold κ (type_interp rti sr τ) se sv)) in "Hrec".
+      replace (eval_kind_se se κ) with (eval_kind se κ); last done.
+      iEval (rewrite Hκ) in "Hrec".
+      iEval (rewrite <- (fold_type_interp_subst se τ κ sκ' sv Hκ)) in "Hrec".
+      iExact "Hrec".
+    - iIntros "[%Hsv Hτrec]".
+      iEval (rewrite type_interp_eq).
+      iExists sκ.
+      iSplit. { iPureIntro. unfold type_skind. simpl. by rewrite Hκ. }
+      iSplit. { iPureIntro. exact Hsv. }
+      iEval (cbn [pre_type_interp]).
+      iEval (rewrite (rec_interp_unfold κ (type_interp rti sr τ) se sv)).
+      replace (eval_kind_se se κ) with (eval_kind se κ); last done.
+      iEval (rewrite Hκ).
+      iEval (rewrite (fold_type_interp_subst se τ κ sκ sv Hκ)) in "Hτrec".
+      iExact "Hτrec".
+  Qed.
+
+  Lemma sem_env_interp_extend_type F (se: semantic_env (Σ:=Σ)) κ sκ T :
+    sem_env_interp F se →
+    eval_kind se κ = Some sκ →
+    skind_has_stype sκ T →
+    sem_env_interp (F <| fc_type_vars ::= cons κ |>) (senv_insert_type sκ T se).
+  Proof.
+    intros [Hkind Htype] Heval Hstype.
+    split.
+    - (* kind_ctx_interp *)
+      unfold kind_ctx_interp in *.
+      destruct Hkind as (Hmem & Hrep & Hsize).
+      repeat split; assumption.
+    - (* type_ctx_interp *)
+      unfold type_ctx_interp in *.
+      simpl.
+      apply Forall2_cons.
+      + split.
+        * rewrite eval_kind_senv_insert_type. by split.
+        * eapply Forall2_impl; first done.
+          intros κ0 [sκ0 T0] [Heval0 Hstype0].
+          rewrite eval_kind_senv_insert_type.
+          split; [exact Heval0 | exact Hstype0].
+  Qed.
 
 End properties.
