theories/iris/logrel/util.v
@@ -1,0 +1,206 @@
+From Stdlib Require Export ZArith.
+
+From stdpp Require Export base list.
+
+Require Export RecordUpdate.RecordUpdate.
+
+From iris.proofmode Require Export base proofmode classes.
+
+From RichWasm.named_props Require Export named_props custom_syntax.
+From RichWasm Require Export layout syntax typing util.
+From RichWasm.compiler Require Export prelude codegen instruction module.
+From RichWasm.iris Require Export autowp memory logrel util wp_codegen.
+Require Export RichWasm.iris.logrel.instr.kinding.
+
+Set Bullet Behavior "Strict Subproofs".
+Set Default Goal Selector "!".
+
+Section common.
+
+  Context `{!logrel_na_invs Σ}.
+  Context `{!wasmG Σ}.
+  Context `{!richwasmG Σ}.
+
+  Lemma eval_rep_emptyenv :
+    forall ρ ιs,
+      eval_rep EmptyEnv ρ = Some ιs ->
+      ∀ (se: semantic_env (Σ:=Σ)),
+        eval_rep se ρ = Some ιs.
+  Proof.
+    induction ρ using rep_ind; intros * Hev *; cbn in Hev; cbn.
+    - inversion Hev.
+    - rewrite -Hev.
+      f_equal.
+      apply fmap_Some in Hev.
+      destruct Hev as (ιss & Hev & _).
+      apply mk_is_Some in Hev.
+      apply mapM_is_Some_1 in Hev.
+      apply Forall_mapM_ext.
+      eapply Forall_impl.
+      { eapply (List.Forall_and H Hev). }
+      cbn.
+      intros ρ [Hev' [ιs' Hempty]].
+      erewrite Hev'; eauto.
+    - rewrite -Hev.
+      f_equal.
+      apply fmap_Some in Hev.
+      destruct Hev as (ιss & Hev & _).
+      apply mk_is_Some in Hev.
+      apply mapM_is_Some_1 in Hev.
+      apply Forall_mapM_ext.
+      eapply Forall_impl.
+      { eapply (List.Forall_and H Hev). }
+      cbn.
+      intros ρ [Hev' [ιs' Hempty]].
+      erewrite Hev'; eauto.
+    - done.
+  Qed.
+
+  Lemma mapM_eval_rep_emptyenv ρs ιss (se: semantic_env (Σ:=Σ)) :
+    mapM (eval_rep EmptyEnv) ρs = Some ιss ->
+    mapM (eval_rep se) ρs = Some ιss.
+  Proof.
+    intros Hemp.
+    rewrite mapM_Some in Hemp.
+    rewrite mapM_Some.
+    eapply Forall2_impl.
+    2: {
+      intros.
+      apply eval_rep_emptyenv.
+      apply H.
+    }
+    done.
+  Qed.
+
+  Lemma sum_offset_emptyenv ρs i off (se: semantic_env (Σ:=Σ)) :
+    sum_offset EmptyEnv ρs i = Some off ->
+    sum_offset se ρs i = Some off.
+  Proof.
+    intros Hso.
+    apply bind_Some in Hso as [ιss [Her H]].
+    eapply mapM_eval_rep_emptyenv in Her.
+    apply bind_Some.
+    eauto.
+  Qed.
+
+  Lemma eval_kind_of_eval_rep (se: semantic_env (Σ:=Σ)) ρ ιs :
+    eval_rep se ρ = Some ιs ->
+    forall ξ, eval_kind se (VALTYPE ρ ξ) = Some (SVALTYPE ιs ξ).
+  Proof.
+    intros Heval ξ.
+    unfold eval_kind.
+    apply bind_Some.
+    by eexists.
+  Qed.
+
+  Lemma type_skind_eval_rep (se: semantic_env (Σ:=Σ)) F ρ ιs ξ τ ιs' ξ' :
+    has_kind F τ (VALTYPE ρ ξ) ->
+    sem_env_interp F se ->
+    eval_rep se ρ = Some ιs ->
+    type_skind se τ = Some (SVALTYPE ιs' ξ') ->
+    ιs = ιs' /\ ξ = ξ'.
+  Proof.
+    intros.
+    assert (SVALTYPE ιs ξ = SVALTYPE ιs' ξ') as Heq.
+    - eapply type_skind_has_kind_agree; try done.
+      cbn.
+      by rewrite H1.
+    - by inversion Heq.
+  Qed.
+
+  Lemma type_skind_eval_rep_emptyenv (se: semantic_env (Σ:=Σ)) F ρ ιs ξ τ ιs' ξ' :
+    has_kind F τ (VALTYPE ρ ξ) ->
+    sem_env_interp F se ->
+    eval_rep EmptyEnv ρ = Some ιs ->
+    type_skind se τ = Some (SVALTYPE ιs' ξ') ->
+    ιs = ιs' /\ ξ = ξ'.
+  Proof.
+    intros.
+    eapply type_skind_eval_rep; try done.
+    by apply eval_rep_emptyenv.
+  Qed.
+
+  Lemma fe_of_context_labels F f :
+    fe_of_context F = fe_of_context (F <| fc_labels ::= f |>).
+  Proof.
+    done.
+  Qed.
+
+  Lemma seq_forall_leq base len :
+    Forall (λ i, i < base + len) (seq base len).
+  Proof.
+    rewrite Forall_seq.
+    intros j Hj.
+    lia.
+  Qed.
+
+  Lemma map_seq_forall_localidx_leq base len :
+    Forall (λ i : prelude.W.localidx, localimm i < base + len)
+      (map prelude.W.Mk_localidx (seq base len)).
+  Proof.
+    apply Forall_map.
+    apply seq_forall_leq.
+  Qed.
+
+  Lemma map_seq_forall_localidx_neq base len :
+    Forall (λ i : prelude.W.localidx, localimm i ≠ base + len)
+      (map prelude.W.Mk_localidx (seq base len)).
+  Proof.
+    eapply Forall_impl; first apply map_seq_forall_localidx_leq.
+    lias.
+  Qed.
+
+  Lemma eval_rep_senv_insert_type sκ T (se: semantic_env (Σ:=Σ)) ρ :
+    eval_rep (senv_insert_type sκ T se) ρ = eval_rep se ρ.
+  Proof.
+    induction ρ using rep_ind; cbn.
+    - reflexivity.
+    - f_equal. apply Forall_mapM_ext.
+      eapply Forall_impl; [exact H |].
+      intros ρ' IH. apply IH.
+    - f_equal. apply Forall_mapM_ext.
+      eapply Forall_impl; [exact H |].
+      intros ρ' IH. apply IH.
+    - reflexivity.
+  Qed.
+
+  Lemma eval_size_senv_insert_type sκ T (se: semantic_env (Σ:=Σ)) σ :
+    eval_size (senv_insert_type sκ T se) σ = eval_size se σ.
+  Proof.
+    induction σ using size_ind; cbn.
+    - reflexivity.
+    - f_equal. apply Forall_mapM_ext.
+      eapply Forall_impl; [exact H |].
+      intros σ' IH. apply IH.
+    - f_equal. apply Forall_mapM_ext. exact H.
+    - by rewrite eval_rep_senv_insert_type.
+    - reflexivity.
+  Qed.
+
+  Lemma eval_kind_senv_insert_type sκ T (se: semantic_env (Σ:=Σ)) κ :
+    eval_kind (senv_insert_type sκ T se) κ = eval_kind se κ.
+  Proof.
+    unfold eval_kind, senv_insert_type. simpl.
+    destruct κ; simpl.
+    - rewrite eval_rep_senv_insert_type. reflexivity.
+    - rewrite eval_size_senv_insert_type. reflexivity.
+  Qed.
+
+  Lemma fe_wlocal_offset_length F :
+    fe_wlocal_offset (fe_of_context F) = length $ concat (typing.fc_locals F).
+  Proof.
+    unfold fe_wlocal_offset. simpl.
+    apply sum_list_with_length_concat.
+  Qed.
+
+  Lemma eval_rep_prod_atoms (se: semantic_env (Σ:=Σ)) ηs :
+    eval_rep se (ProdR (map (AtomR ∘ prim_to_arep) ηs)) = Some (map prim_to_arep ηs).
+  Proof.
+    induction ηs; simpl; first done.
+    simpl in IHηs.
+    destruct (mapM (eval_rep se) (map (AtomR ∘ prim_to_arep) ηs)) as [ιss|] eqn:Hmapм; simpl in *; last done.
+    injection IHηs as IHηs.
+    by rewrite IHηs.
+  Qed.
+
+End common.
